src/DY.Core.Label.fst
@@ -1,51 +1,88 @@
 module DY.Core.Label
 
+open DY.Core.Bytes.Type
 open DY.Core.Label.Type
 open DY.Core.Trace.Type
 
+class label_description_flow = {
+  get_description: content:bytes -> bytes;
+  desc_can_flow: bytes -> bytes -> prop;
+  desc_can_flow_refl: x:bytes -> Lemma (x `desc_can_flow` x);
+  desc_can_flow_trans: x:bytes -> y:bytes -> z:bytes ->
+    Lemma
+    (requires x `desc_can_flow` y /\ y `desc_can_flow` z)
+    (ensures x `desc_can_flow` z);
+}
+
+val description_order:
+  {|label_description_flow|} ->
+  DY.Core.Label.Lattice.order bytes
+let description_order #ldf = {
+  rel = (fun x y -> desc_can_flow y x);
+  refl = (fun x -> desc_can_flow_refl x);
+  trans = (fun x y z ->
+    desc_can_flow_trans z y x
+  );
+}
+
 val pre_can_flow:
-  pre_pre_label -> pre_pre_label -> prop
-let pre_can_flow who1 who2 =
-  who2 `pre_pre_label_order.rel` who1
+  {|label_description_flow|} ->
+  pre_pre_label bytes -> pre_pre_label bytes -> prop
+let pre_can_flow #ldf who1 who2 =
+  who2 `(pre_pre_label_order description_order).rel` who1
+
+val pre_can_flow_refl:
+  {|label_description_flow|} ->
+  who:pre_pre_label bytes ->
+  Lemma
+  (ensures who `pre_can_flow` who)
+  [SMTPat (who `pre_can_flow` who)]
+let pre_can_flow_refl #ldf who =
+  (pre_pre_label_order description_order).refl who
 
 val pre_can_flow_transitive:
-  who1:pre_pre_label -> who2:pre_pre_label -> who3:pre_pre_label ->
+  {|label_description_flow|} ->
+  who1:pre_pre_label bytes -> who2:pre_pre_label bytes -> who3:pre_pre_label bytes ->
   Lemma
   (requires who1 `pre_can_flow` who2 /\ who2 `pre_can_flow` who3)
   (ensures who1 `pre_can_flow` who3)
   [SMTPat (who1 `pre_can_flow` who2); SMTPat (who1 `pre_can_flow` who3)]
-let pre_can_flow_transitive who1 who2 who3 =
-  pre_pre_label_order.trans who3 who2 who1
+let pre_can_flow_transitive #ldf who1 who2 who3 =
+  (pre_pre_label_order description_order).trans who3 who2 who1
 
-val is_corrupt: trace -> pre_pre_label -> prop
-let is_corrupt tr who =
-  exists prin sess_id.
-    who `pre_can_flow` (S prin sess_id) /\
-    was_corrupt tr prin sess_id
+val is_corrupt: {|label_description_flow|} -> trace -> pre_pre_label bytes -> prop
+let is_corrupt #ldf tr who =
+  exists prin content.
+    who `pre_can_flow` (S prin (get_description content)) /\
+    state_was_corrupt tr prin content
 
 val is_corrupt_later:
+  {|label_description_flow|} ->
   tr1:trace -> tr2:trace ->
-  who:pre_pre_label ->
+  who:pre_pre_label bytes ->
   Lemma
   (requires is_corrupt tr1 who /\ tr1 <$ tr2)
   (ensures is_corrupt tr2 who)
   [SMTPat (is_corrupt tr1 who); SMTPat (tr1 <$ tr2)]
-let is_corrupt_later tr1 tr2 who = ()
+let is_corrupt_later #ldf tr1 tr2 who = ()
 
 val is_corrupt_order:
+  {|label_description_flow|} ->
   tr:trace ->
-  who1:pre_pre_label -> who2:pre_pre_label ->
+  who1:pre_pre_label bytes -> who2:pre_pre_label bytes ->
   Lemma
   (requires is_corrupt tr who1 /\ who2 `pre_can_flow` who1)
   (ensures is_corrupt tr who2)
   // TODO SMT pattern is weird, refactor
-  [SMTPat (is_corrupt tr who1); SMTPat (who1 `pre_pre_label_order.rel` who2)]
-let is_corrupt_order tr who1 who2 = ()
+  [SMTPat (is_corrupt tr who1); SMTPat (who1 `(pre_pre_label_order description_order).rel` who2)]
+let is_corrupt_order #ldf tr who1 who2 = ()
+
+type label = label bytes
 
 [@@"opaque_to_smt"]
-val can_flow: trace -> label -> label -> prop
-let can_flow tr l1 l2 =
-  l2 `(label_order (is_corrupt tr)).rel` l1
+val can_flow: {|label_description_flow|} -> trace -> label -> label -> prop
+let can_flow #ldf tr l1 l2 =
+  l2 `(label_order description_order (is_corrupt tr)).rel` l1
 
 [@@"opaque_to_smt"]
 val secret: label
@@ -73,18 +110,18 @@ let principal_label prin =
   DY.Core.Label.Lattice.Leaf (State (P prin))
 
 [@@"opaque_to_smt"]
-val principal_state_label: principal -> nat -> label
+val principal_state_label: principal -> bytes -> label
 let principal_state_label prin sess_id =
   DY.Core.Label.Lattice.Leaf (State (S prin sess_id))
 
 [@@"opaque_to_smt"]
-val principal_corrupt: trace -> principal -> prop
-let principal_corrupt tr prin =
+val principal_corrupt: {|label_description_flow|} -> trace -> principal -> prop
+let principal_corrupt #ldf tr prin =
   is_corrupt tr (P prin)
 
 [@@"opaque_to_smt"]
-val principal_state_corrupt: trace -> principal -> nat -> prop
-let principal_state_corrupt tr prin sess_id =
+val principal_state_corrupt: {|label_description_flow|} -> trace -> principal -> bytes -> prop
+let principal_state_corrupt #ldf tr prin sess_id =
   is_corrupt tr (S prin sess_id)
 
 val principal_label_injective:
@@ -97,7 +134,7 @@ let principal_label_injective p1 p2 =
   normalize_term_spec principal_label
 
 val principal_state_label_injective:
-  p1:principal -> s1:nat -> p2:principal -> s2:nat ->
+  p1:principal -> s1:bytes -> p2:principal -> s2:bytes ->
   Lemma
   (requires principal_state_label p1 s1 == principal_state_label p2 s2)
   (ensures p1 == p2 /\ s1 == s2)
@@ -106,138 +143,162 @@ let principal_state_label_injective p1 s1 p2 s2 =
   normalize_term_spec principal_state_label
 
 val principal_corrupt_later:
+  {|label_description_flow|} ->
   tr1:trace -> tr2:trace ->
   prin:principal ->
   Lemma
   (requires principal_corrupt tr1 prin /\ tr1 <$ tr2)
   (ensures principal_corrupt tr2 prin)
   [SMTPat (principal_corrupt tr1 prin); SMTPat (tr1 <$ tr2)]
-let principal_corrupt_later tr1 tr2 prin =
+let principal_corrupt_later #ldf tr1 tr2 prin =
   assert_norm(principal_corrupt tr1 prin == is_corrupt tr1 (P prin));
   assert_norm(principal_corrupt tr2 prin == is_corrupt tr2 (P prin))
 
 val principal_state_corrupt_later:
+  {|label_description_flow|} ->
   tr1:trace -> tr2:trace ->
-  prin:principal -> sess_id:nat ->
+  prin:principal -> sess_id:bytes ->
   Lemma
   (requires principal_state_corrupt tr1 prin sess_id /\ tr1 <$ tr2)
   (ensures principal_state_corrupt tr2 prin sess_id)
   [SMTPat (principal_state_corrupt tr1 prin sess_id); SMTPat (tr1 <$ tr2)]
-let principal_state_corrupt_later tr1 tr2 prin sess_id =
+let principal_state_corrupt_later #ldf tr1 tr2 prin sess_id =
   assert_norm(principal_state_corrupt tr1 prin sess_id == is_corrupt tr1 (S prin sess_id));
   assert_norm(principal_state_corrupt tr2 prin sess_id == is_corrupt tr2 (S prin sess_id))
 
+val state_was_corrupt_implies_principal_state_corrupt:
+  {|label_description_flow|} ->
+  tr:trace ->
+  prin:principal -> content:bytes ->
+  Lemma
+  (requires state_was_corrupt tr prin content)
+  (ensures principal_state_corrupt tr prin (get_description content))
+  [SMTPat (state_was_corrupt tr prin content); SMTPat (principal_state_corrupt tr prin (get_description content))]
+let state_was_corrupt_implies_principal_state_corrupt #ldf tr prin content =
+  assert_norm(principal_state_corrupt tr prin (get_description content) == is_corrupt tr (S prin (get_description content)))
+
 val can_flow_reflexive:
+  {|label_description_flow|} ->
   tr:trace -> l:label ->
   Lemma
   (ensures l `can_flow tr` l)
   [SMTPat (l `can_flow tr` l)]
-let can_flow_reflexive tr l =
+let can_flow_reflexive #ldf tr l =
   normalize_term_spec can_flow;
-  (label_order (is_corrupt tr)).refl l
+  (label_order description_order (is_corrupt tr)).refl l
 
 val can_flow_transitive:
+  {|label_description_flow|} ->
   tr:trace -> l1:label -> l2:label -> l3:label ->
   Lemma
   (requires l1 `can_flow tr` l2 /\ l2 `can_flow tr` l3)
   (ensures l1 `can_flow tr` l3)
   [SMTPat (l1 `can_flow tr` l3); SMTPat (l1 `can_flow tr` l2)]
-let can_flow_transitive tr l1 l2 l3 =
+let can_flow_transitive #ldf tr l1 l2 l3 =
   normalize_term_spec can_flow;
-  (label_order (is_corrupt tr)).trans l3 l2 l1
+  (label_order description_order (is_corrupt tr)).trans l3 l2 l1
 
 val can_flow_later:
+  {|label_description_flow|} ->
   tr1:trace -> tr2:trace ->
   l1:label -> l2:label ->
   Lemma
   (requires l1 `can_flow tr1` l2 /\ tr1 <$ tr2)
   (ensures l1 `can_flow tr2` l2)
   [SMTPat (l1 `can_flow tr1` l2); SMTPat (tr1 <$ tr2)]
-let can_flow_later tr1 tr2 l1 l2 =
+let can_flow_later #ldf tr1 tr2 l1 l2 =
   normalize_term_spec can_flow;
-  DY.Core.Label.Lattice.lattice_order_monotone (pre_label_order pre_pre_label_order (is_corrupt tr1)) (pre_label_order pre_pre_label_order (is_corrupt tr2)) l2 l1
+  DY.Core.Label.Lattice.lattice_order_monotone (pre_label_order (pre_pre_label_order description_order) (is_corrupt tr1)) (pre_label_order (pre_pre_label_order description_order) (is_corrupt tr2)) l2 l1
 
 val secret_is_bottom:
+  {|label_description_flow|} ->
   tr:trace -> l:label ->
   Lemma
   (ensures l `can_flow tr` secret)
   [SMTPat (l `can_flow tr` secret)]
-let secret_is_bottom tr l =
+let secret_is_bottom #ldf tr l =
   normalize_term_spec can_flow;
   normalize_term_spec secret;
-  DY.Core.Label.Lattice.bottom_to_bottom (pre_label_order pre_pre_label_order (is_corrupt tr)) Secret l
+  DY.Core.Label.Lattice.bottom_to_bottom (pre_label_order (pre_pre_label_order description_order) (is_corrupt tr)) Secret l
 
 val public_is_top:
+  {|label_description_flow|} ->
   tr:trace -> l:label ->
   Lemma
   (ensures public `can_flow tr` l)
   [SMTPat (public `can_flow tr` l)]
-let public_is_top tr l =
+let public_is_top #ldf tr l =
   normalize_term_spec can_flow;
   normalize_term_spec public;
-  DY.Core.Label.Lattice.top_to_top (pre_label_order pre_pre_label_order (is_corrupt tr)) Public l
+  DY.Core.Label.Lattice.top_to_top (pre_label_order (pre_pre_label_order description_order) (is_corrupt tr)) Public l
 
 val meet_eq:
+  {|label_description_flow|} ->
   tr:trace -> x:label -> y1:label -> y2:label ->
   Lemma
   (ensures meet y1 y2 `can_flow tr` x <==> (y1 `can_flow tr` x /\ y2 `can_flow tr` x))
   [SMTPat (meet y1 y2 `can_flow tr` x)] //Not sure about this
-let meet_eq tr x y1 y2 =
+let meet_eq #ldf tr x y1 y2 =
   normalize_term_spec can_flow;
   normalize_term_spec meet;
-  DY.Core.Label.Lattice.meet_eq (pre_label_order pre_pre_label_order (is_corrupt tr)) x y1 y2
+  DY.Core.Label.Lattice.meet_eq (pre_label_order (pre_pre_label_order description_order) (is_corrupt tr)) x y1 y2
 
 val join_eq:
+  {|label_description_flow|} ->
   tr:trace -> x1:label -> x2:label -> y:label ->
   Lemma
   (ensures y `can_flow tr` join x1 x2 <==> (y `can_flow tr` x1 /\ y `can_flow tr` x2))
   [SMTPat (y `can_flow tr` join x1 x2)] //Not sure about this
-let join_eq tr x1 x2 y =
+let join_eq #ldf tr x1 x2 y =
   normalize_term_spec can_flow;
   normalize_term_spec join;
-  DY.Core.Label.Lattice.join_eq (pre_label_order pre_pre_label_order (is_corrupt tr)) x1 x2 y
+  DY.Core.Label.Lattice.join_eq (pre_label_order (pre_pre_label_order description_order) (is_corrupt tr)) x1 x2 y
 
 val principal_flow_to_public_eq:
+  {|label_description_flow|} ->
   tr:trace -> prin:principal ->
   Lemma
   (ensures (principal_label prin) `can_flow tr` public <==> principal_corrupt tr prin)
   [SMTPat ((principal_label prin) `can_flow tr` public)] //Not sure about this
-let principal_flow_to_public_eq tr prin =
+let principal_flow_to_public_eq #ldf tr prin =
   normalize_term_spec can_flow;
   normalize_term_spec principal_label;
   normalize_term_spec public;
   assert_norm(principal_corrupt tr prin == is_corrupt tr (P prin));
-  DY.Core.Label.Lattice.leaf_eq (pre_label_order pre_pre_label_order (is_corrupt tr)) Public (State (P prin))
+  DY.Core.Label.Lattice.leaf_eq (pre_label_order (pre_pre_label_order description_order) (is_corrupt tr)) Public (State (P prin))
 
 val principal_state_flow_to_public_eq:
-  tr:trace -> prin:principal -> sess_id:nat ->
+  {|label_description_flow|} ->
+  tr:trace -> prin:principal -> sess_id:bytes ->
   Lemma
   (ensures (principal_state_label prin sess_id) `can_flow tr` public <==> principal_state_corrupt tr prin sess_id)
   [SMTPat ((principal_state_label prin sess_id) `can_flow tr` public)] //Not sure about this
-let principal_state_flow_to_public_eq tr prin sess_id =
+let principal_state_flow_to_public_eq #ldf tr prin sess_id =
   normalize_term_spec can_flow;
   normalize_term_spec principal_state_label;
   normalize_term_spec public;
   assert_norm(principal_state_corrupt tr prin sess_id == is_corrupt tr (S prin sess_id));
-  DY.Core.Label.Lattice.leaf_eq (pre_label_order pre_pre_label_order (is_corrupt tr)) Public (State (S prin sess_id))
+  DY.Core.Label.Lattice.leaf_eq (pre_label_order (pre_pre_label_order description_order) (is_corrupt tr)) Public (State (S prin sess_id))
 
 val principal_flow_to_principal_state:
-  tr:trace -> prin:principal -> sess_id:nat ->
+  {|label_description_flow|} ->
+  tr:trace -> prin:principal -> sess_id:bytes ->
   Lemma
   (ensures (principal_label prin) `can_flow tr` (principal_state_label prin sess_id))
   [SMTPat ((principal_label prin) `can_flow tr` (principal_state_label prin sess_id))]
-let principal_flow_to_principal_state tr prin sess_id =
+let principal_flow_to_principal_state #ldf tr prin sess_id =
   normalize_term_spec can_flow;
   normalize_term_spec principal_label;
   normalize_term_spec principal_state_label
 
 val join_flow_to_public_eq:
+  {|label_description_flow|} ->
   tr:trace -> x1:label -> x2:label ->
   Lemma
   (ensures (join x1 x2) `can_flow tr` public <==> x1 `can_flow tr` public \/ x2 `can_flow tr` public)
   [SMTPat ((join x1 x2) `can_flow tr` public)] //Not sure about this
-let join_flow_to_public_eq tr x1 x2 =
+let join_flow_to_public_eq #ldf tr x1 x2 =
   normalize_term_spec can_flow;
   normalize_term_spec join;
   normalize_term_spec public;
-  DY.Core.Label.Lattice.leaf_less_join (pre_label_order pre_pre_label_order (is_corrupt tr)) Public x1 x2
+  DY.Core.Label.Lattice.leaf_less_join (pre_label_order (pre_pre_label_order description_order) (is_corrupt tr)) Public x1 x2
